removed explicit call for implicit parameters, lemma renames and split larger lemmas up

FYP/Graph/Path.lean
@@ -10,23 +10,23 @@ instance {n : ℕ} : Membership (Fin n) (Path n) :=
 
 -- A path is valid if every consecutive pair of vertices
 -- has an edge in the graph.
-def validPath {n : ℕ} (G : Graph n) : Path n → Prop
+def validPath (G : Graph n) : Path n → Prop
   | [] => False
   | [_] => True
   | (u :: v :: rest) =>
       G.w u v ≠ ⊤ ∧ validPath G (v :: rest)
 
-def pathStart {n : ℕ} : Path n → Option (Fin n)
+def pathStart : Path n → Option (Fin n)
   | [] => none
   | v :: _ => some v
 
-def pathEnd {n : ℕ} : Path n → Option (Fin n)
+def pathEnd : Path n → Option (Fin n)
   | [] => none
   | [v] => some v
   | _ :: rest => pathEnd rest
 
 -- Compute weight of a path by summing edge weights
-def pathWeight {n : ℕ} (G : Graph n) : Path n → ℕ∞
+def pathWeight (G : Graph n) : Path n → ℕ∞
   | [] => 0
   | [_] => 0  -- single vertex has weight 0
   | (u :: v :: rest) =>
@@ -36,16 +36,16 @@ def pathWeight {n : ℕ} (G : Graph n) : Path n → ℕ∞
 @[simp] lemma pathWeight_cons (u v : Fin n) (rest : Path n) :
   pathWeight G (u :: v :: rest) = G.w u v + pathWeight G (v :: rest) := rfl
 
-def isPathFromTo {n : ℕ} (G : Graph n) (p : Path n) (i j : Fin n) : Prop :=
+def isPathFromTo (G : Graph n) (p : Path n) (i j : Fin n) : Prop :=
   validPath G p ∧
   pathStart p = some i ∧
   pathEnd p = some j
 
 -- defines distance as the minimum weight over all paths from i to j
-noncomputable def shortestDist {n : ℕ} (G : Graph n) (i j : Fin n) : ℕ∞ :=
+noncomputable def shortestDist (G : Graph n) (i j : Fin n) : ℕ∞ :=
   sInf {w | ∃ p, isPathFromTo G p i j ∧ pathWeight G p = w}
 
-noncomputable def distUpToList {n : ℕ} (G : Graph n) (l : List (Fin n)) (i j : Fin n) : ℕ∞ :=
+noncomputable def distUpToList (G : Graph n) (l : List (Fin n)) (i j : Fin n) : ℕ∞ :=
   sInf {w | ∃ p,
     isPathFromTo G p i j ∧
     (∀ v ∈ p, v ∈ l ∨ v = i ∨ v = j) ∧
