FYP/FloydWarshall/Lemmas.lean
@@ -6,25 +6,24 @@ import FYP.FloydWarshall.HelperLemmas
 
 namespace FYP
 
-lemma initDist_eq_sInf_eq {n : ℕ} (G : Graph n) (j : Fin n) :
- initDist G j j =
-  sInf {w | ∃ p, isPathFromTo G p j j ∧
+lemma initDist_eq_sInf_diag (j : Fin n) :
+ initDist G j j = sInf {w | ∃ p,
+            isPathFromTo G p j j ∧
             (∀ v ∈ p, v = j) ∧
             pathWeight G p = w} := by
   apply le_antisymm
-  · -- show initDist G j j ≤ sInf ...
+  · -- initDist G j j ≤ sInf ...
     simp [initDist]  -- initDist G j j = 0
-  · -- show sInf ... ≤ initDist G j j
+  · -- sInf ... ≤ initDist G j j
     apply sInf_le
-    -- pick the path [j]
     refine ⟨[j], ⟨?_, ?_, ?_⟩⟩
-    · simp only [isPathFromTo, validPath, pathStart, pathEnd, and_self]
+    · simp [isPathFromTo, validPath, pathStart, pathEnd]
     · intro v hv
       rw [List.mem_singleton] at hv
       rw [hv]
     · simp [initDist]
 
-lemma initDist_le_sInf_neq_by_path_witness {n : ℕ} (G : Graph n) (i j : Fin n) (h : i ≠ j) :
+lemma initDist_le_sInf_neq (i j : Fin n) (h : i ≠ j) :
   initDist G i j ≤
     sInf {w | ∃ p, isPathFromTo G p i j ∧
             (∀ v ∈ p, v = i ∨ v = j) ∧ pathWeight G p = w} := by
@@ -77,11 +76,11 @@ lemma initDist_le_sInf_neq_by_path_witness {n : ℕ} (G : Graph n) (i j : Fin n)
           rw [<- hy_j]
           simp
 
-lemma initDist_eq_sInf_neq {n : ℕ} (G : Graph n) (i j : Fin n) (h : i ≠ j) :
+lemma initDist_eq_sInf_offdiag (i j : Fin n) (h : i ≠ j) :
   initDist G i j = sInf {w | ∃ p, isPathFromTo G p i j ∧ (∀ v ∈ p, v = i ∨ v = j)
                      ∧ pathWeight G p = w} := by
   apply le_antisymm
-  · exact initDist_le_sInf_neq_by_path_witness G i j h
+  · exact initDist_le_sInf_neq i j h
   · apply sInf_le
     refine ⟨[i, j], ⟨?path_valid, ?path_start, ?path_end⟩, ?verts⟩
     · simp [validPath]
@@ -95,17 +94,16 @@ lemma initDist_eq_sInf_neq {n : ℕ} (G : Graph n) (i j : Fin n) (h : i ≠ j) :
 -- Initial distance function is the same as the shortest distance
 -- considering only paths that use vertices in the empty list
 -- This is the base case for the induction in fw_invariant
-lemma initDist_eq_sInf {n : ℕ} (G : Graph n) (i j : Fin n) :
+lemma initDist_eq_sInf (i j : Fin n) :
   initDist G i j = distUpToList G [] i j := by
   simp only [distUpToList, List.not_mem_nil, false_or]
   by_cases h : i = j
   · simp only [h, or_self]
-    exact initDist_eq_sInf_eq G j
-  · exact initDist_eq_sInf_neq G i j h
+    exact initDist_eq_sInf_diag j
+  · exact initDist_eq_sInf_offdiag i j h
 
-lemma distUpToList_le_of_path {n : ℕ} (G : Graph n)
-  (ks : List (Fin n)) (i j : Fin n) (p : Path n)
-  (hp_path : isPathFromTo G p i j)
+lemma distUpToList_le_of_path (ks : List (Fin n)) (i j : Fin n)
+  (p : Path n) (hp_path : isPathFromTo G p i j)
   (hp_verts : ∀ v ∈ p, v ∈ ks ∨ v = i ∨ v = j) :
   distUpToList G ks i j ≤ pathWeight G p := by
     unfold distUpToList
@@ -114,7 +112,7 @@ lemma distUpToList_le_of_path {n : ℕ} (G : Graph n)
 
 -- adding a vertex to the list of intermediate vertices is a monotone operation
 -- i.e. it can only decrease distances
-lemma distUpToList_mono {n : ℕ} (G : Graph n) (ks1 ks2 : List (Fin n))
+lemma distUpToList_mono (ks1 ks2 : List (Fin n))
   (h : ∀ v, v ∈ ks1 → v ∈ ks2) :
   ∀ i j , distUpToList G ks2 i j ≤ distUpToList G ks1 i j := by
   intro i j
@@ -124,19 +122,19 @@ lemma distUpToList_mono {n : ℕ} (G : Graph n) (ks1 ks2 : List (Fin n))
   rw [<- hp_weight]
   have hp_vertices_ks2 : ∀ v ∈ p, v ∈ ks2 ∨ v = i ∨ v = j := by
       exact fun v a ↦ Or.imp_left (h v) (hp_vertices v a)
-  exact distUpToList_le_of_path G ks2 i j p hp_path hp_vertices_ks2
+  exact distUpToList_le_of_path ks2 i j p hp_path hp_vertices_ks2
 
 -- normally an infimum is not guaranteed to be attained, but in this case
 -- we are restricted to only positive integer weights so the infimum is actually a minimum
-lemma exists_path_weight_eq_distUpToList {n : ℕ} (G : Graph n) (ks : List (Fin n)) (i j : Fin n) :
-  ∃ p, isPathFromTo G p i j ∧ (∀ v ∈ p, v ∈ ks)
+lemma exists_path_weight_eq_distUpToList (ks : List (Fin n)) (i j : Fin n) :
+  ∃ p, isPathFromTo G p i j ∧ (∀ v ∈ p, v ∈ ks) -- ∨ v = i ∨ v = j)
       ∧ pathWeight G p = distUpToList G ks i j := by
     unfold distUpToList
     sorry
 
 -- any path from i to j that can use k is less than
 -- or equal to the path that goes via k
-lemma fwStep_le_split {n : ℕ} (G : Graph n) (ks : List (Fin n)) (k i j : Fin n) :
+lemma fwStep_le_split (ks : List (Fin n)) (k i j : Fin n) :
   distUpToList G (k :: ks) i j ≤ distUpToList G ks i k + distUpToList G ks k j := by
   -- apply infimum lemma
   unfold distUpToList
@@ -144,9 +142,9 @@ lemma fwStep_le_split {n : ℕ} (G : Graph n) (ks : List (Fin n)) (k i j : Fin n
   · refine ⟨0, ?_⟩
     intro w hw
     exact zero_le _
-  · rcases exists_path_weight_eq_distUpToList G ks i k with
+  · rcases exists_path_weight_eq_distUpToList ks i k with
       ⟨p1, hp1_path, hp1_verts, hp1_w⟩
-    rcases exists_path_weight_eq_distUpToList G ks k j with
+    rcases exists_path_weight_eq_distUpToList ks k j with
       ⟨p2, hp2_path, hp2_verts, hp2_w⟩
     -- define concatenation
     let p := p1 ++ p2.tail
@@ -173,120 +171,130 @@ lemma fwStep_le_split {n : ℕ} (G : Graph n) (ks : List (Fin n)) (k i j : Fin n
         simp [hend2, pathEnd_eq]
     · intro v hv
       unfold p at hv
-      apply List.mem_append.mp at hv
-      cases hv with
+      cases List.mem_append.mp hv with
       | inl hv1 =>
-          have : v ∈ ks := hp1_verts v hv1
-          exact Or.inl (List.mem_cons_of_mem _ this)
+          have h := hp1_verts v hv1
+          simp[h]
       | inr hv2 =>
-          have : v ∈ p2 := List.mem_of_mem_tail hv2
-          have : v ∈ ks := hp2_verts v this
-          exact Or.inl (List.mem_cons_of_mem _ this)
+          have hv2' : v ∈ p2 := List.mem_of_mem_tail hv2
+          have h := hp2_verts v hv2'
+          simp [h]
     · simp only [distUpToList] at hp1_w hp2_w
       rw [<- hp1_w, <- hp2_w]
       unfold p
       rw [pathWeight_append_tail p1 p2 hvalid1 h_link]
 
+lemma fwStep_lower_bound_p1 (ks : List (Fin n)) (k i j : Fin n)
+  (p : Path n) (hp_path : isPathFromTo G p i j)
+  (hp_verts : ∀ v ∈ p, v ∈ k :: ks)
+  (hp_weight : pathWeight G p = distUpToList G (k :: ks) i j)
+  (h : k ∈ p) :
+  min (distUpToList G ks i j)
+    (distUpToList G ks i k + distUpToList G ks k j) ≤
+      distUpToList G (k :: ks) i j := by
+    let p1 := p.takeWhile (fun v => v ≠ k)
+    let p2 := p.drop (p1.length + 1)
+    have hp_split : p = p1 ++ [k] ++ p2 :=
+      takeWhile_drop_split k p h
+    simp only [hp_split] at hp_path
+    have split_prefix := isPathFromTo_prefix p1 p2 i j k hp_path
+    have split_suffix := isPathFromTo_suffix p1 p2 i j k hp_path
+    have hp_verts_p1 : ∀ v ∈ p1 ++ [k], v ∈ ks ∨ v = i ∨ v = k := by
+      intros v hv;
+      simp only [List.mem_cons] at hp_verts
+      have hv_p : v ∈ p := by
+        have : v ∈ p1 ++ [k] ++ p2 := by
+          apply List.mem_append.mpr
+          exact Or.inl hv
+        simpa [hp_split] using this
+      specialize hp_verts v hv_p
+      cases hp_verts with
+      | inl hk => exact Or.inr (Or.inr hk)
+      | inr hks => exact Or.inl hks
+    have h1 : distUpToList G ks i k ≤ pathWeight G (p1 ++ [k]) :=
+      distUpToList_le_of_path ks i k (p1 ++ [k])
+        (split_prefix) (hp_verts_p1)
+    have hp_verts_p2 : ∀ v ∈ ([k] ++ p2), v ∈ ks ∨ v = k ∨ v = j := by
+      intros v hv
+      have hv_p : v ∈ p := by
+        have : v ∈ p1 ++ [k] ++ p2 := by
+          apply List.mem_append.mpr
+          simp only [List.cons_append, List.mem_cons] at hv
+          cases hv with
+          | inl hk =>
+            subst hk
+            simp
+          | inr hv_p2 =>
+            right
+            exact hv_p2
+        simpa [hp_split] using this
+      specialize hp_verts v hv_p
+      simp only [List.mem_cons] at hp_verts
+      cases hp_verts with
+      | inl hk => exact Or.inr (Or.inl hk)
+      | inr hks => exact Or.inl hks
+    have h2 : distUpToList G ks k j ≤ pathWeight G ([k] ++ p2) := by
+      exact distUpToList_le_of_path ks k j ([k] ++ p2)
+        (split_suffix) hp_verts_p2
+    have hp_sum :
+      pathWeight G p = pathWeight G (p1 ++ [k]) + pathWeight G ([k] ++ p2) := by
+        have h_valid : validPath G (p1 ++ [k]) := by
+          simp [isPathFromTo] at hp_path
+          exact validPath_prefix p1 p2 k (by simp [hp_path.left])
+        have h_end : pathEnd (p1 ++ [k]) = pathStart ([k] ++ p2) := by
+          simp [pathEnd_append p1 [k] (by simp), pathStart, pathEnd]
+        rw [<- pathWeight_append_tail (p1 ++ [k]) ([k] ++ p2) h_valid h_end]
+        simp [hp_split]
+    -- transitivity
+    have h_total : distUpToList G ks i k + distUpToList G ks k j ≤ pathWeight G p := by
+      simp only [hp_sum]
+      exact add_le_add h1 h2
+    have h_right :
+      distUpToList G ks i k + distUpToList G ks k j
+        ≤ distUpToList G (k :: ks) i j := by
+      simpa [hp_weight] using h_total
+    exact le_trans (min_le_right _ _) h_right
+
 -- any path from i to j that can use k is at least as long as the
 -- shorter of the path that doesn't use k and the path that goes via k
-lemma min_le_list_with_k {n : ℕ} (G : Graph n) (ks : List (Fin n)) (k i j : Fin n) :
+lemma fwStep_lower_bound (ks : List (Fin n)) (k i j : Fin n) :
   min (distUpToList G ks i j) (distUpToList G ks i k + distUpToList G ks k j) ≤
     distUpToList G (k :: ks) i j := by
     obtain ⟨p, hp_path, hp_verts, hp_weight⟩ :=
-      exists_path_weight_eq_distUpToList G (k :: ks) i j
+      exists_path_weight_eq_distUpToList (k :: ks) i j
     by_cases h : k ∈ p
-    · -- any path from i to j that uses k can be split into
+    · -- path from i to j that uses k can be split into
       -- a path from i to k and a path from k to j
-      let p1 := p.takeWhile (fun v => v ≠ k)
-      let p2 := p.drop (p1.length + 1)
-      have hp_split : p = p1 ++ [k] ++ p2 :=
-        takeWhile_drop_split k p h
-      simp only [hp_split] at hp_path
-      have split_prefix := isPathFromTo_prefix p1 p2 i j k hp_path
-      have split_suffix := isPathFromTo_suffix p1 p2 i j k hp_path
-      have hp_verts_p1 : ∀ v ∈ p1 ++ [k], v ∈ ks ∨ v = i ∨ v = k := by
-        intros v hv;
-        simp only [List.mem_cons] at hp_verts
-        have hv_p : v ∈ p := by
-          have : v ∈ p1 ++ [k] ++ p2 := by
-            apply List.mem_append.mpr
-            exact Or.inl hv
-          simpa [hp_split] using this
-        specialize hp_verts v hv_p
-        cases hp_verts with
-        | inl hk => exact Or.inr (Or.inr hk)
-        | inr hks => exact Or.inl hks
-      have h1 : distUpToList G ks i k ≤ pathWeight G (p1 ++ [k]) :=
-        distUpToList_le_of_path G ks i k (p1 ++ [k])
-          (split_prefix) (hp_verts_p1)
-      have hp_verts_p2 : ∀ v ∈ ([k] ++ p2), v ∈ ks ∨ v = k ∨ v = j := by
-        intros v hv
-        have hv_p : v ∈ p := by
-          have : v ∈ p1 ++ [k] ++ p2 := by
-            apply List.mem_append.mpr
-            simp only [List.cons_append, List.mem_cons] at hv
-            cases hv with
-            | inl hk =>
-              subst hk
-              left
-              simp
-            | inr hv_p2 =>
-              right
-              exact hv_p2
-          simpa [hp_split] using this
-        specialize hp_verts v hv_p
-        simp only [List.mem_cons] at hp_verts
-        cases hp_verts with
-        | inl hk => exact Or.inr (Or.inl hk)
-        | inr hks => exact Or.inl hks
-      have h2 : distUpToList G ks k j ≤ pathWeight G ([k] ++ p2) := by
-        exact distUpToList_le_of_path G ks k j ([k] ++ p2)
-          (split_suffix) hp_verts_p2
-      have hp_sum :
-        pathWeight G p = pathWeight G (p1 ++ [k]) + pathWeight G ([k] ++ p2) := by
-          have h_valid : validPath G (p1 ++ [k]) := by
-            simp [isPathFromTo] at hp_path
-            exact validPath_prefix p1 p2 k (by simp [hp_path.left])
-          have h_end : pathEnd (p1 ++ [k]) = pathStart ([k] ++ p2) := by
-            simp [pathEnd_append p1 [k] (by simp), pathStart, pathEnd]
-          rw [<- pathWeight_append_tail (p1 ++ [k]) ([k] ++ p2) h_valid h_end]
-          simp [hp_split]
-      -- transitivity
-      have h_total : distUpToList G ks i k + distUpToList G ks k j ≤ pathWeight G p := by
-        simp only [hp_sum]
-        exact add_le_add h1 h2
-      have h_right :
-        distUpToList G ks i k + distUpToList G ks k j
-          ≤ distUpToList G (k :: ks) i j := by
-        simpa [hp_weight] using h_total
-      exact le_trans (min_le_right _ _) h_right
+      exact fwStep_lower_bound_p1 ks k i j p hp_path hp_verts hp_weight h
     · -- case 2: p doesn't use k
       -- any path from i to j that doesn't use k is still a valid path
       -- when we add k to the list of intermediate vertices
       have hp_verts_ks : ∀ v ∈ p, v ∈ ks ∨ v = i ∨ v = j := by
         intro v hv
         have hmem := hp_verts v hv
-        rcases List.mem_cons.mp hmem with h' | h'
-        · subst h'
-          exact False.elim (h hv)
-        · exact Or.inl h'
+        have hv_ne_k : v ≠ k := by
+          intro hvk
+          subst hvk
+          exact h hv
+        simp [hv_ne_k] at hmem
+        simp [hmem]
       have hA :
         distUpToList G ks i j ≤ pathWeight G p :=
-        distUpToList_le_of_path G ks i j p hp_path hp_verts_ks
+        distUpToList_le_of_path ks i j p hp_path hp_verts_ks
       have h1 := (min_le_left (distUpToList G ks i j)
         (distUpToList G ks i k + distUpToList G ks k j)).trans hA
       rw [hp_weight] at h1
       exact h1
 
 -- proof for adding vertex k to the list of intermediate vertices
-lemma fwStep_invariant {n : ℕ} (G : Graph n) (ks : List (Fin n)) (k i j : Fin n) :
+lemma fwStep_invariant (ks : List (Fin n)) (k i j : Fin n) :
   min (distUpToList G ks i j) (distUpToList G ks i k + distUpToList G ks k j)
     = distUpToList G (k :: ks) i j := by
   apply le_antisymm
   · -- lower bound: show min ... ≤ distUpToList G (k :: ks) i j
     -- i.e. any path from i to j that can use k is at least as long as the shorter of
     -- the path that doesn't use k and the path that goes via k
-    exact min_le_list_with_k G ks k i j
+    exact fwStep_lower_bound ks k i j
   · -- upper bound: show distUpToList G (k :: ks) i j ≤ min ...
     apply le_min
     · -- show distUpToList G (k :: ks) i j ≤ distUpToList G ks i j
@@ -294,10 +302,10 @@ lemma fwStep_invariant {n : ℕ} (G : Graph n) (ks : List (Fin n)) (k i j : Fin 
       have subsetofList : ∀ v, v ∈ ks → v ∈ k :: ks := by
         intro v hv
         exact List.mem_cons_of_mem k hv
-      exact distUpToList_mono G ks (k :: ks) subsetofList i j
+      exact distUpToList_mono ks (k :: ks) subsetofList i j
     · -- show distUpToList G (k :: ks) i j ≤ distUpToList G ks i k + distUpToList G ks k j
       -- i.e. any path from i to j that can use k can be split into
       -- a path from i to k and a path from k to j
-      exact fwStep_le_split G ks k i j
+      exact fwStep_le_split ks k i j
 
 end FYP
